bedrock2/src/ZNamesSyntax.v
@@ -1,11 +1,9 @@
 Require Import Coq.ZArith.ZArith.
 Require Import bedrock2.Syntax.
-Require Import bedrock2.Basic_bopnames.
 
 Definition ZNames : Syntax.parameters := {|
   Syntax.varname := Z;
   Syntax.funname := Z;
 
   Syntax.actname := Empty_set;
-  Syntax.bopname := bopname;
 |}.
